integrate Gencot_ESArray* into Gencot_CArray*

isa/Gencot_CArray_Lemmas.thy
@@ -180,7 +180,7 @@ theorem errsem_setArr:
   setArrFxd (a,i,v) = (a,())"
   by (simp add: setArrFxd_def setArr'_def vldArr fld_inverse)
 
-definition ctrct_modifyArrFxd :: "'arr \<times> ('m::len) word \<times> ('el \<times> 'arg \<Rightarrow> 'el \<times> 'arg) \<times> 'arg \<Rightarrow> bool"
+definition ctrct_modifyArrFxd :: "'arr \<times> ('m::len) word \<times> ('el \<times> 'arg \<Rightarrow> 'el \<times> 'out) \<times> 'arg \<Rightarrow> bool"
   where ctrct_modifyArrFxd_def[simp]:
   "ctrct_modifyArrFxd x \<equiv> let (a,i,f,v) = x in vldFxd a (unat i)"
 theorem sem_modifyArr:
@@ -190,23 +190,10 @@ theorem sem_modifyArr:
   by (simp add: modifyArrFxd_def modifyArr'_def split_def Let_def vldArr lstFxd_def arrFxd_def elm_updateFxd_def elmFxd_def)
 theorem errsem_modifyArr:
  "\<not> ctrct_modifyArrFxd (a,i,f,x) ==> 
-  modifyArrFxd (a,i,f,x) = (a, x)"
+  modifyArrFxd (a,i,f,x) = modifyArrFxd (a,0,f,x)"
   by (simp add: modifyArrFxd_def modifyArr'_def vldArr fld_inverse)
 
-definition ctrct_modifyArrDfltFxd :: "'arr \<times> ('m::len) word \<times> ('el \<times> 'arg \<Rightarrow> 'el \<times> 'out) \<times> 'arg \<Rightarrow> bool"
-  where ctrct_modifyArrDfltFxd_def[simp]:
-  "ctrct_modifyArrDfltFxd x \<equiv> let (a,i,f,v) = x in vldFxd a (unat i)"
-theorem sem_modifyArrDflt:
- "ctrct_modifyArrDfltFxd (a,i,f,x) ==> 
-  modifyArrDfltFxd (a,i,f,x) = 
-  (let (e,y) = f (elmFxd (unat i) a, x) in (elm_updateFxd (unat i) (\<lambda>_.e) a, y))"
-  by (simp add: modifyArrDfltFxd_def modifyArrDflt'_def split_def Let_def vldArr lstFxd_def arrFxd_def elm_updateFxd_def elmFxd_def)
-theorem errsem_modifyArrDflt:
- "\<not> ctrct_modifyArrDfltFxd (a,i,f,x) ==>
-  modifyArrDfltFxd (a,i,f,x) = (a, defaultVal ())"
-  by (simp add: modifyArrDfltFxd_def modifyArrDflt'_def vldArr fld_inverse)
-
-definition ctrct_modrefArrFxd :: "'arr \<times> ('m::len) word \<times> ('pel \<times> 'arg \<Rightarrow> 'pel \<times> 'arg) \<times> 'arg \<Rightarrow> bool"
+definition ctrct_modrefArrFxd :: "'arr \<times> ('m::len) word \<times> ('pel \<times> 'arg \<Rightarrow> 'pel \<times> 'out) \<times> 'arg \<Rightarrow> bool"
   where ctrct_modrefArrFxd_def[simp]:
   "ctrct_modrefArrFxd x \<equiv> let (a,i,f,v) = x in vldFxd a (unat i)"
 theorem sem_modrefArr:
@@ -216,22 +203,161 @@ theorem sem_modrefArr:
   by (simp add: modrefArrFxd_def modrefArr'_def split_def Let_def vldArr lstFxd_def arrFxd_def elm_updateFxd_def elmFxd_def)
 theorem errsem_modrefArr:
  "\<not> ctrct_modrefArrFxd (a,i,f,x) ==> 
-  modrefArrFxd (a,i,f,x) = (a, x)"
+  modrefArrFxd (a,i,f,x) = modrefArrFxd (a,0,f,x)"
   by (simp add: modrefArrFxd_def modrefArr'_def vldArr fld_inverse)
 
-definition ctrct_modrefArrDfltFxd :: "'arr \<times> ('m::len) word \<times> ('pel \<times> 'arg \<Rightarrow> 'pel \<times> 'out) \<times> 'arg \<Rightarrow> bool"
-  where ctrct_modrefArrDfltFxd_def[simp]:
-  "ctrct_modrefArrDfltFxd x \<equiv> let (a,i,f,v) = x in vldFxd a (unat i)"
-theorem sem_modrefArrDflt:
- "ctrct_modrefArrDfltFxd (a,i,f,x) ==> 
-  modrefArrDfltFxd (a,i,f,x) = 
-  (let (e,y) = f (toPtr (elmFxd (unat i) a), x) in (elm_updateFxd (unat i) (\<lambda>_.frPtr e) a, y))"
-  by (simp add: modrefArrDfltFxd_def modrefArrDflt'_def split_def Let_def vldArr lstFxd_def arrFxd_def elm_updateFxd_def elmFxd_def)
-theorem errsem_modrefArrDflt:
- "\<not> ctrct_modrefArrDfltFxd (a,i,f,x) ==>
-  modrefArrDfltFxd (a,i,f,x) = (a, defaultVal ())"
-  by (simp add: modrefArrDfltFxd_def modrefArrDflt'_def vldArr fld_inverse)
-
 end
+
+text \<open>Extend the overloaded abstract data type to explicitly sized arrays.
+      Additionally introduce the following function for filling an array 
+      with an explicitly specified size.\<close>
+consts 
+  arr_fill_n :: "nat \<Rightarrow> (nat \<Rightarrow> 'el) \<Rightarrow> 'arr"
+
+text \<open>Wellformedness predicate for explicitly sized arrays:\<close>
+definition wlfES :: "'el CArrES\<^sub>T \<Rightarrow> bool"
+  where wlfES_def[simp]: "wlfES a \<equiv> 
+    length (fst a) = (unat (snd a)) \<and> length (fst a) > 0"
+
+text \<open>Define the abstract data type functions for explicitly sized arrays.
+The explicit size is ignored and the intrinsic size of the list is used.\<close>
+definition sizES :: "'el CArrPtr\<^sub>T \<Rightarrow> nat"
+  where "sizES a \<equiv> length a"
+definition vldES :: "'el CArrPtr\<^sub>T \<Rightarrow> nat \<Rightarrow> bool"
+  where "vldES a i \<equiv> i < sizES a"
+definition elmES :: "nat \<Rightarrow> 'el CArrPtr\<^sub>T \<Rightarrow> 'el"
+  where "elmES i a \<equiv> nth a i"
+definition elm_updateES :: "nat \<Rightarrow> ('el \<Rightarrow> 'el) \<Rightarrow> 'el CArrPtr\<^sub>T \<Rightarrow> 'el CArrPtr\<^sub>T"
+  where "elm_updateES i f a \<equiv> (list_update a i (f (elmES i a)))"
+definition elm_modifiedES :: "nat \<Rightarrow> ('el \<Rightarrow> 'el \<Rightarrow> bool) \<Rightarrow> 'el CArrPtr\<^sub>T \<Rightarrow> 'el CArrPtr\<^sub>T \<Rightarrow> bool"
+  where elm_modified_defES: "elm_modifiedES i m a1 a2 \<equiv> 
+    m (elmES i a1) (elmES i a2) \<and> (\<forall>j \<noteq> i. vldES a1 j \<longrightarrow> elmES j a1 = elmES j a2)"
+definition arr_fill_nES :: "nat \<Rightarrow> (nat \<Rightarrow> 'el) \<Rightarrow> 'el CArrPtr\<^sub>T"
+  where "arr_fill_nES n f \<equiv> [f x . x \<leftarrow> [0 ..< n]]"
+
+text \<open>Laws for the abstract data type functions\<close>
+lemma sizArrES: "sizES a = length a"
+  by (simp add:sizES_def)
+lemma vldArrES: "vldES a n = (n < length a)"
+  by (simp add: vldES_def sizArrES)
+lemma elm_identUpdES[simp]: "elm_updateES i (\<lambda>a. a) = (\<lambda>a. a)"
+  apply (unfold elm_updateES_def)
+  by(simp add: elmES_def)
+lemma elm_sameUpdES: "elm_updateES i (\<lambda>_. m (elmES i x)) x = elm_updateES i m x"
+  by(simp add: elm_updateES_def)
+thm list_update_same_conv
+lemma elm_distUpdES: "vldES a i \<Longrightarrow> (elm_updateES i f) ( (elm_updateES i g) a) = elm_updateES i (f \<circ> g) a"
+  for f:: "'el \<Rightarrow> 'el" and a::"'el CArrPtr\<^sub>T"
+  apply (unfold elm_updateES_def elmES_def fst_def vldArrES)
+  by(auto)
+lemma elm_commUpd_elmES: "i < j \<Longrightarrow> (elm_updateES j m2) \<circ> (elm_updateES i m1) = (elm_updateES i m1) \<circ> (elm_updateES j m2)"
+  apply (unfold elm_updateES_def elmES_def)
+  apply(rule ext,simp)
+  apply(rule list_update_swap)
+  by(simp)
+lemma elmElmUpdES: "vldES a i \<Longrightarrow> elmES i (elm_updateES i f a) = f (elmES i a)"
+  by(auto simp add: elm_updateES_def elmES_def vldArrES)
+lemma elmElmUpdFrameES: "vldES a i \<and> vldES a j \<and> i \<noteq> j \<Longrightarrow> elmES j (elm_updateES i f a) = elmES j a"
+  by(auto simp add: elm_updateES_def elmES_def vldArrES)
+lemma elmArrFillES: "i < n \<Longrightarrow> elmES i (arr_fill_nES n f) = f i"
+  by(auto simp add: elmES_def arr_fill_nES_def vldArrES)
+lemma sizArrFill: "sizES (arr_fill_nES n f) = n"
+  by(auto simp add: arr_fill_nES_def sizArrES)
+
+text \<open>Array equality by extensionality. \<close>
+lemma eqArrES: "sizES a1 = sizES a2 \<Longrightarrow>
+              (a1 = a2) = 
+              (\<forall> i. (vldES a1 i) \<longrightarrow> ((elmES i a1) = (elmES i a2)))"
+  for a1::"'el CArrPtr\<^sub>T" and a2::"'el CArrPtr\<^sub>T"
+  apply(rule iffI)
+   apply(rule allI)
+   apply(rule impI)
+   apply(auto simp add: elmES_def vldArrES sizArrES)
+  apply(case_tac a1)
+  apply(case_tac a2)
+  apply(auto)
+  apply(rule nth_equalityI)
+  by(auto)
+
+lemma eqElmUpdES: "sizES a1 = sizES a2 \<Longrightarrow> vldES a2 i \<Longrightarrow> (a1 = elm_updateES i f a2) =
+                 ((elmES i a1) = f (elmES i a2) \<and> (\<forall> j. j \<noteq> i \<and> (vldES a1 j) \<longrightarrow> (elmES j a1) = (elmES j a2)))"
+  apply(rule iffI)
+   apply(auto)
+    apply(subst elmElmUpdES,auto)
+  apply(subst elmElmUpdFrameES,auto simp add: vldArrES sizArrES)
+  apply(subst eqArrES)
+    apply(auto simp add:elm_updateES_def)
+   apply(auto simp add: elmES_def sizArrES)
+  apply(case_tac "ia = i")
+   apply(simp)
+  by(auto simp add: vldArrES)
+lemma eqArrFillES: "sizES a = n \<Longrightarrow> (a = arr_fill_nES n f) = 
+                 ((\<forall> i. (vldES a i) \<longrightarrow> ((elmES i a) = f i)))"
+  apply(rule iffI)
+   apply(auto)
+   apply(rule elmArrFillES)
+   apply(simp add: vldArrES arr_fill_nES_def sizArrES)
+  apply(subst eqArrES)
+   apply(simp add: vldArrES arr_fill_nES_def sizArrES)
+   apply(simp add: arr_fill_nES_def)
+   apply(rule allI)
+   apply(rule impI)
+  by (auto simp add: elmES_def vldArrES sizArrES)
+
+text \<open>Semantics theorems for the Gencot array functions.\<close>
+lemma "a \<noteq> [] \<Longrightarrow> hd a = a ! 0"
+  sorry
+definition ctrct_getArrES :: "'el CArrES\<^sub>T \<times> ('m::len) word \<Rightarrow> bool"
+  where ctrct_getArrES_def[simp]:
+  "ctrct_getArrES x \<equiv> let ((a,n),i) = x in (unat i) < (unat n)"
+theorem sem_getArrES: 
+ "wlfES a \<and> ctrct_getArrES (a,i) \<Longrightarrow> 
+  getArrES (a,i) = elmES (unat i) (fst a)"
+  by (auto simp add: getArrES_def elmES_def)
+theorem errsem_getArrES:
+ "wlfES a \<and> \<not> ctrct_getArrES (a,i) \<Longrightarrow> 
+  getArrES (a,i) = elmES 0 (fst a)"
+  apply(simp add: getArrES_def vldArrES elmES_def split_def)
+  by(rule hd_conv_nth,simp)
+
+definition ctrct_setArrES :: "'el CArrES\<^sub>T \<times> ('m::len) word \<times> 'el \<Rightarrow> bool"
+  where ctrct_setArrES_def[simp]:
+  "ctrct_setArrES x \<equiv> let ((a,n),i,v) = x in (unat i) < (unat n)"
+theorem sem_setArrES: 
+ "wlfES a \<and> ctrct_setArrES (a,i,v) \<Longrightarrow> 
+  setArrES (a,i,v) = ((elm_updateES (unat i) (\<lambda>_.v) (fst a),(snd a)), ())"
+  by (auto simp add: setArrES_def elm_updateES_def)
+theorem errsem_setArrES:
+ "wlfES a \<and> \<not> ctrct_setArrES (a,i,v) \<Longrightarrow> 
+  setArrES (a,i,v) = (a,())"
+  by (simp add: setArrES_def split_def)
+
+definition ctrct_modifyArrES :: "'el CArrES\<^sub>T \<times> ('m::len) word \<times> ('el \<times> 'arg \<Rightarrow> 'el \<times> 'out) \<times> 'arg \<Rightarrow> bool"
+  where ctrct_modifyArrES_def[simp]:
+  "ctrct_modifyArrES x \<equiv> let ((a,n),i,f,v) = x in (unat i) < (unat n)"
+theorem sem_modifyArrES:
+ "wlfES a \<and> ctrct_modifyArrES (a,i,f,x) \<Longrightarrow> 
+  modifyArrES (a,i,f,x) = 
+  (let (e,y) = f (elmES (unat i) (fst a), x) 
+  in ((elm_updateES (unat i) (\<lambda>_.e) (fst a),(snd a)), y))"
+  by (simp add: modifyArrES_def split_def Let_def elm_updateES_def elmES_def)
+theorem errsem_modifyArrES:
+ "wlfES a \<and> \<not> ctrct_modifyArrES (a,i,f,x) ==> 
+  modifyArrES (a,i,f,x) = modifyArrES (a,0,f,x)"
+  by (simp add: modifyArrES_def split_def)
+
+definition ctrct_modrefArrES :: "'el CArrES\<^sub>T \<times> ('m::len) word \<times> ('pel \<times> 'arg \<Rightarrow> 'pel \<times> 'out) \<times> 'arg \<Rightarrow> bool"
+  where ctrct_modrefArrES_def[simp]:
+  "ctrct_modrefArrES x \<equiv> let ((a,n),i,f,v) = x in (unat i) < (unat n)"
+theorem sem_modrefArrES:
+ "wlfES a \<and> ctrct_modrefArrES (a,i,f,x) \<Longrightarrow> 
+  modrefArrES (a,i,f,x) = 
+  (let (e,y) = f (toPtr (elmES (unat i) (fst a)), x) 
+  in ((elm_updateES (unat i) (\<lambda>_.frPtr e) (fst a),(snd a)), y))"
+  by (simp add: modrefArrES_def split_def Let_def elm_updateES_def elmES_def)
+theorem errsem_modrefArrES:
+ "wlfES a \<and> \<not> ctrct_modrefArrES (a,i,f,x) ==> 
+  modrefArrES (a,i,f,x) = modrefArrES (a,0,f,x)"
+  by (simp add: modrefArrES_def split_def)
 
 end
