isa/Gencot_CArray_Tuples.thy
@@ -24,33 +24,25 @@ definition setArr' :: "('n::len, 'el) FixedList \<Rightarrow> 'idx::len word \<R
       if unat idx >= LENGTH('n) then lst
       else (Abs_FixedList (list_update (Rep_FixedList lst) (unat idx) elm))"
 
-definition modifyArr' :: "('n::len, 'el) FixedList \<Rightarrow> 'idx::len word \<Rightarrow> ('el \<times> 'arg \<Rightarrow> 'el \<times> 'arg) \<Rightarrow> 'arg \<Rightarrow> ('n, 'el) FixedList \<times> 'arg"
+definition modifyArr' :: "('n::len, 'el) FixedList \<Rightarrow> 'idx::len word \<Rightarrow> ('el \<times> 'arg \<Rightarrow> 'el \<times> 'out) \<Rightarrow> 'arg \<Rightarrow> ('n, 'el) FixedList \<times> 'out"
   where
     "modifyArr' lst idx chf inp \<equiv> 
-      if unat idx >= LENGTH('n) then (lst, inp)
-      else let l = Rep_FixedList lst; elm = nth l (unat idx); chres = chf(elm, inp)
-        in (Abs_FixedList (list_update l (unat idx) (fst chres)), snd chres)"
+      let i = (if unat idx >= LENGTH('n) then 0 else unat idx); 
+          l = Rep_FixedList lst; elm = nth l i; chres = chf(elm, inp)
+      in (Abs_FixedList (list_update l i (fst chres)), snd chres)"
 
-definition modifyArrDflt' :: "('n::len, 'el) FixedList \<Rightarrow> 'idx::len word \<Rightarrow> ('el \<times> 'arg \<Rightarrow> 'el \<times> 'out) \<Rightarrow> 'arg \<Rightarrow> ('n, 'el) FixedList \<times> 'out"
-  where
-    "modifyArrDflt' lst idx chf inp \<equiv> 
-      if unat idx >= LENGTH('n) then (lst, defaultVal ())
-      else let l = Rep_FixedList lst; elm = nth l (unat idx); chres = chf(elm, inp)
-        in (Abs_FixedList (list_update l (unat idx) (fst chres)), snd chres)"
-
-definition modrefArr' :: "('n::len, 'el) FixedList \<Rightarrow> 'idx::len word \<Rightarrow> ('pel \<times> 'arg \<Rightarrow> 'pel \<times> 'arg) \<Rightarrow> 'arg \<Rightarrow> ('n, 'el) FixedList \<times> 'arg"
+definition modrefArr' :: "('n::len, 'el) FixedList \<Rightarrow> 'idx::len word \<Rightarrow> ('pel \<times> 'arg \<Rightarrow> 'pel \<times> 'out) \<Rightarrow> 'arg \<Rightarrow> ('n, 'el) FixedList \<times> 'out"
   where
     "modrefArr' lst idx chf inp \<equiv> 
-      if unat idx >= LENGTH('n) then (lst, inp)
-      else let l = Rep_FixedList lst; elm = nth l (unat idx); chres = chf(toPtr elm, inp)
-        in (Abs_FixedList (list_update l (unat idx) (frPtr (fst chres))), snd chres)"
+      let i = (if unat idx >= LENGTH('n) then 0 else unat idx); 
+          l = Rep_FixedList lst; elm = nth l i; chres = chf(toPtr elm, inp)
+      in (Abs_FixedList (list_update l i (frPtr (fst chres))), snd chres)"
 
-definition modrefArrDflt' :: "('n::len, 'el) FixedList \<Rightarrow> 'idx::len word \<Rightarrow> ('pel \<times> 'arg \<Rightarrow> 'pel \<times> 'out) \<Rightarrow> 'arg \<Rightarrow> ('n, 'el) FixedList \<times> 'out"
-  where
-    "modrefArrDflt' lst idx chf inp \<equiv> 
-      if unat idx >= LENGTH('n) then (lst, defaultVal ())
-      else let l = Rep_FixedList lst; elm = nth l (unat idx); chres = chf(toPtr elm, inp)
-        in (Abs_FixedList (list_update l (unat idx) (frPtr (fst chres))), snd chres)"
+definition toCAES' :: "('n::len, 'el) FixedList \<Rightarrow> 'el CArrES\<^sub>T"
+  where "toCAES' lst \<equiv> (Rep_FixedList lst, of_nat LENGTH('n))"
+
+definition fromCAES' :: "'el CArrES\<^sub>T \<Rightarrow> ('n::len, 'el) FixedList"
+  where "fromCAES' aes \<equiv> Abs_FixedList (fst aes) "
 
 text \<open>For every actual wrapper record the following locale will be interpreted.
       It takes the wrapper record access and constructor as parameters.
@@ -66,19 +58,50 @@ definition getArrFxd :: "'arr \<times> ('m::len) word \<Rightarrow> 'el"
   where "getArrFxd arg \<equiv> let (arr,idx) = arg in getArr' (fld arr) idx"
 definition setArrFxd :: "'arr \<times> ('m::len) word \<times> 'el \<Rightarrow> 'arr \<times> unit"
   where "setArrFxd arg \<equiv> let (arr,idx,elm) = arg in (wrp(setArr' (fld arr) idx elm), ())"
-definition modifyArrFxd :: "'arr \<times> ('m::len) word \<times> ('el \<times> 'arg \<Rightarrow> 'el \<times> 'arg) \<times> 'arg \<Rightarrow> 'arr \<times> 'arg"
+definition modifyArrFxd :: "'arr \<times> ('m::len) word \<times> ('el \<times> 'arg \<Rightarrow> 'el \<times> 'out) \<times> 'arg \<Rightarrow> 'arr \<times> 'out"
   where "modifyArrFxd arg \<equiv> let (arr, idx, chf, inp) = arg; 
     (reslst,res) = modifyArr' (fld arr) idx chf inp in (wrp reslst, res)"
-definition modifyArrDfltFxd :: "'arr \<times> ('m::len) word \<times> ('el \<times> 'arg \<Rightarrow> 'el \<times> 'out) \<times> 'arg \<Rightarrow> 'arr \<times> 'out"
-  where "modifyArrDfltFxd arg \<equiv> let (arr, idx, chf, inp) = arg;
-    (reslst,res) = modifyArrDflt' (fld arr) idx chf inp in (wrp reslst, res)"
-definition modrefArrFxd :: "'arr \<times> ('m::len) word \<times> ('pel \<times> 'arg \<Rightarrow> 'pel \<times> 'arg) \<times> 'arg \<Rightarrow> 'arr \<times> 'arg"
+definition modrefArrFxd :: "'arr \<times> ('m::len) word \<times> ('pel \<times> 'arg \<Rightarrow> 'pel \<times> 'out) \<times> 'arg \<Rightarrow> 'arr \<times> 'out"
   where "modrefArrFxd arg \<equiv> let (arr, idx, chf, inp) = arg; 
     (reslst,res) = modrefArr' (fld arr) idx chf inp in (wrp reslst, res)"
-definition modrefArrDfltFxd :: "'arr \<times> ('m::len) word \<times> ('pel \<times> 'arg \<Rightarrow> 'pel \<times> 'out) \<times> 'arg \<Rightarrow> 'arr \<times> 'out"
-  where "modrefArrDfltFxd arg \<equiv> let (arr, idx, chf, inp) = arg;
-    (reslst,res) = modrefArrDflt' (fld arr) idx chf inp in (wrp reslst, res)"
+
+definition toCAESFxd :: "'arr \<Rightarrow> 'el CArrES\<^sub>T"
+  where "toCAESFxd arr \<equiv> toCAES' (fld arr)"
+definition fromCAESFxd :: "'el CArrES\<^sub>T \<Rightarrow> 'arr"
+  where "fromCAESFxd aes \<equiv> wrp (fromCAES' aes)"
 
 end
+
+text \<open>Define the array functions for explicitly sized arrays\<close>
+
+definition getArrES :: "'el CArrES\<^sub>T \<times> 'idx::len word \<Rightarrow> 'el"
+  where 
+    "getArrES arg \<equiv>
+      let ((lst,len),idx) = arg
+      in if unat idx >= unat len then hd lst
+         else (nth lst (unat idx))"
+
+definition setArrES :: "'el CArrES\<^sub>T \<times> 'idx::len word \<times> 'el \<Rightarrow> 'el CArrES\<^sub>T \<times> unit"
+  where
+    "setArrES arg \<equiv> 
+      let ((lst,len),idx,elm) = arg
+      in if unat idx >= unat len then ((lst,len),())
+         else (((list_update lst (unat idx) elm),len),())"
+
+definition modifyArrES :: "'el CArrES\<^sub>T \<times> ('idx::len word \<times> ('el \<times> 'arg \<Rightarrow> 'el \<times> 'out) \<times> 'arg) \<Rightarrow> 'el CArrES\<^sub>T \<times> 'out"
+  where
+    "modifyArrES arg \<equiv> 
+      let ((lst,len),(idx,chf,inp)) = arg;
+          i = (if unat idx < unat len then (unat idx) else 0);
+          elm = nth lst i; chres = chf(elm, inp)
+      in ((list_update lst i (fst chres),len), snd chres)"
+
+definition modrefArrES :: "'el CArrES\<^sub>T \<times> ('idx::len word \<times> ('pel \<times> 'arg \<Rightarrow> 'pel \<times> 'out) \<times> 'arg) \<Rightarrow> 'el CArrES\<^sub>T \<times> 'out"
+  where
+    "modrefArrES arg \<equiv> 
+      let ((lst,len),(idx,chf,inp)) = arg;
+          i = (if unat idx < unat len then (unat idx) else 0);
+          elm = nth lst i; chres = chf(toPtr elm, inp)
+      in ((list_update lst i (frPtr (fst chres)),len), snd chres)"
 
 end
