isa/Gencot_ESArray.thy
@@ -1,7 +1,0 @@
-theory Gencot_ESArray
-  imports ShallowShared
-begin
-
-(* not yet implemented *)
-
-end
